renamed spec_refines to letrec_refines; finished proving the necessary metatheory about it

theories/Ref/SpecRefines.v
@@ -20,6 +20,7 @@ From EnTree Require Import
      Basics.QuantType
      Core.EnTreeDefinition
      Core.SubEvent
+     Ref.Padded
      Ref.EnTreeSpecDefinition
      Ref.EnTreeSpecFacts
      Ref.EnTreeSpecCombinatorFacts
@@ -42,7 +43,7 @@ Definition SpecM' (E:EncType) stack A : Type :=
   entree_spec' (FunStackE E stack) A.
 
 
-Section refines.
+Section lr_refines.
 
 Context {E1 E2 : EncType} {stk1 stk2 : FunStack} {R1 R2 : Type}.
 Context (funs1 : FrameTuple E1 stk1) (funs2 : FrameTuple E2 stk2).
@@ -51,70 +52,295 @@ Context (RPre : Rel (FunStackE E1 stk1) (FunStackE E2 stk2))
   (RPost : PostRel (FunStackE E1 stk1) (FunStackE E2 stk2))
   (RR : R1 -> R2 -> Prop).
 
-Inductive spec_refinesF (sim : SpecM E1 stk1 R1 -> SpecM E2 stk2 R2 -> Prop) : SpecM' E1 stk1 R1 -> SpecM' E2 stk2 R2 -> Prop :=
+Inductive lr_refinesF (sim : SpecM E1 stk1 R1 -> SpecM E2 stk2 R2 -> Prop) : SpecM' E1 stk1 R1 -> SpecM' E2 stk2 R2 -> Prop :=
 
 (* Ret |= Ret *)
-| spec_refinesF_Ret r1 r2 : RR r1 r2 -> spec_refinesF sim (RetF r1) (RetF r2)
+| lr_refinesF_Ret r1 r2 : RR r1 r2 -> lr_refinesF sim (RetF r1) (RetF r2)
 
 (* t1 |= t2 => Tau t1 |= Tau t2 *)
-| spec_refinesF_Tau t1 t2 : sim t1 t2 -> spec_refinesF sim (TauF t1) (TauF t2)
+| lr_refinesF_Tau t1 t2 : sim t1 t2 -> lr_refinesF sim (TauF t1) (TauF t2)
 
 (* RPre e1 e2 -> (forall a b, RPost e1 e2 a b -> k1 a |= k2 b) ->
    Vis e1 k1 |= Vis e2 k2 *)
-| spec_refinesF_Vis e1 e2 k1 k2 : RPre e1 e2 -> (forall a b, RPost e1 e2 a b -> sim (k1 a) (k2 b) ) ->
-                               spec_refinesF sim (VisF (Spec_vis e1) k1) (VisF (Spec_vis e2) k2)
+| lr_refinesF_Vis e1 e2 k1 k2 :
+  RPre e1 e2 -> (forall a b, RPost e1 e2 a b -> sim (k1 a) (k2 b)) ->
+  lr_refinesF sim (VisF (Spec_vis e1) k1) (VisF (Spec_vis e2) k2)
 
 (* t1 |= t2 => Tau t1 |= t2 *)
-| spec_refinesF_TauL t1 ot2 : spec_refinesF sim (observe t1) ot2 ->
-                              spec_refinesF sim (TauF t1) ot2
+| lr_refinesF_TauL t1 ot2 : lr_refinesF sim (observe t1) ot2 ->
+                            lr_refinesF sim (TauF t1) ot2
 
 (* t1 |= t2 => t1 |= Tau t2 *)
-| spec_refinesF_TauR ot1 t2 : spec_refinesF sim ot1 (observe t2) ->
-                              spec_refinesF sim ot1 (TauF t2)
+| lr_refinesF_TauR ot1 t2 : lr_refinesF sim ot1 (observe t2) ->
+                            lr_refinesF sim ot1 (TauF t2)
 
 (* (forall a, t1 |= k a) => t1 |= Forall k *)
-| spec_refinesF_forallR A ot1 k : (forall a, spec_refinesF sim ot1 (observe (k a))) ->
-                                  spec_refinesF sim ot1 (VisF (Spec_forall A) k)
+| lr_refinesF_forallR A ot1 k : (forall a, lr_refinesF sim ot1 (observe (k a))) ->
+                                lr_refinesF sim ot1 (VisF (Spec_forall A) k)
 
 (* (exists a, t1 |= k a) => t1 |= Exists k *)
-| spec_refinesF_existsR A ot1 k a : spec_refinesF sim ot1 (observe (k a)) ->
-                                    spec_refinesF sim ot1 (VisF (Spec_exists A) k)
+| lr_refinesF_existsR A ot1 k a : lr_refinesF sim ot1 (observe (k a)) ->
+                                  lr_refinesF sim ot1 (VisF (Spec_exists A) k)
 
 (* (exists a, k a |= t2) => Forall k |= t2 *)
-| spec_refinesF_forallL A ot2 k a : spec_refinesF sim (observe (k a)) ot2 ->
-                                    spec_refinesF sim (VisF (Spec_forall A) k ) ot2
+| lr_refinesF_forallL A ot2 k a : lr_refinesF sim (observe (k a)) ot2 ->
+                                  lr_refinesF sim (VisF (Spec_forall A) k) ot2
 
 (* (forall a, k a |= t2) => Exists k |= t2 *)
-| spec_refinesF_existsL A ot2 k : (forall a, spec_refinesF sim (observe (k a)) ot2) -> spec_refinesF sim (VisF (Spec_exists A) k) ot2
+| lr_refinesF_existsL A ot2 k : (forall a, lr_refinesF sim (observe (k a)) ot2) ->
+                                lr_refinesF sim (VisF (Spec_exists A) k) ot2
 
 (* apply funs1 call1 >>= k1 |= t2 => CallS call1 >>= k1 |= t2 *)
-| spec_refinesF_unfoldL call1 k1 ot2 :
-    spec_refinesF sim (observe (applyFrameTuple E1 stk1 funs1 call1 >>= k1)) ot2 ->
-    spec_refinesF sim (VisF (Spec_vis (inl call1)) k1) ot2
+| lr_refinesF_unfoldL call1 k1 ot2 :
+    lr_refinesF sim (TauF (applyFrameTuple E1 stk1 funs1 call1 >>= k1)) ot2 ->
+    lr_refinesF sim (VisF (Spec_vis (inl call1)) k1) ot2
 
 (* t1 |= apply funs2 call2 >>= k2 => t1 |= CallS call2 >>= k2 *)
-| spec_refinesF_unfoldR ot1 call2 k2 :
-    spec_refinesF sim ot1 (observe (applyFrameTuple E2 stk2 funs2 call2 >>= k2)) ->
-    spec_refinesF sim ot1 (VisF (Spec_vis (inl call2)) k2)
+| lr_refinesF_unfoldR ot1 call2 k2 :
+    lr_refinesF sim ot1 (TauF (applyFrameTuple E2 stk2 funs2 call2 >>= k2)) ->
+    lr_refinesF sim ot1 (VisF (Spec_vis (inl call2)) k2)
 .
 
-Hint Constructors spec_refinesF : entree_spec.
 
-Definition spec_refines_ sim : SpecM E1 stk1 R1 -> SpecM E2 stk2 R2 -> Prop :=
-  fun t1 t2 => spec_refinesF sim (observe t1) (observe t2).
+(** The standard Paco nonsense **)
 
-Lemma monotone_spec_refinesF ot1 ot2 sim sim' (LE : sim <2= sim')
-      (IN : spec_refinesF sim ot1 ot2) : spec_refinesF sim' ot1 ot2.
+Hint Constructors lr_refinesF : entree_spec.
+
+Definition lr_refines_ sim : SpecM E1 stk1 R1 -> SpecM E2 stk2 R2 -> Prop :=
+  fun t1 t2 => lr_refinesF sim (observe t1) (observe t2).
+
+Lemma monotone_lr_refinesF ot1 ot2 sim sim' (LE : sim <2= sim')
+      (IN : lr_refinesF sim ot1 ot2) : lr_refinesF sim' ot1 ot2.
 Proof with eauto with entree_spec.
   induction IN...
 Qed.
 
-Lemma monotone_spec_refines_: monotone2 spec_refines_.
-Proof. red. intros. eapply monotone_spec_refinesF; eauto. Qed.
+Lemma monotone_lr_refines_: monotone2 lr_refines_.
+Proof. red. intros. eapply monotone_lr_refinesF; eauto. Qed.
 
-Hint Resolve monotone_spec_refines_ : paco.
+(* lr_refines is the coinductive closure of lr_refinesF *)
+Definition lr_refines := paco2 lr_refines_ bot2.
 
-Definition refines := paco2 spec_refines_ bot2.
+(* letrec_refines is the padded version of lr_refines *)
+Definition letrec_refines t1 t2 := lr_refines (pad t1) (pad t2).
 
-End refines.
+End lr_refines.
 
+Global Hint Resolve monotone_lr_refines_ : paco.
+
+Global Instance eq_itree_lr_refines_Proper1 {E1 E2 : EncType} {stk1 stk2} {R1 R2}
+  funs1 funs2 RPre RPost RR r :
+  Proper (eq_itree eq ==> eq_itree eq ==> flip impl)
+    (@lr_refines_ E1 E2 stk1 stk2 R1 R2 funs1 funs2 RPre RPost RR (upaco2 (lr_refines_ funs1 funs2 RPre RPost RR) r)).
+Proof.
+  repeat intro. apply bisimulation_is_eq in H. apply bisimulation_is_eq in H0.
+  subst. auto.
+Qed.
+
+Global Instance eq_itree_lr_refines_Proper2 {E1 E2 : EncType} {stk1 stk2} {R1 R2}
+  funs1 funs2 RPre RPost RR r :
+  Proper (eq_itree eq ==> eq_itree eq ==> flip impl)
+    (paco2 (@lr_refines_ E1 E2 stk1 stk2 R1 R2 funs1 funs2 RPre RPost RR) r).
+Proof.
+  repeat intro. apply bisimulation_is_eq in H. apply bisimulation_is_eq in H0.
+  subst. auto.
+Qed.
+
+
+
+Section lr_refines_props.
+
+Context {E1 E2 : EncType} {stk1 stk2 : FunStack} {R1 R2 : Type} {RR : Rel R1 R2}.
+Context (funs1 : FrameTuple E1 stk1) (funs2 : FrameTuple E2 stk2).
+
+(* Lift a relation on FunStackE events from the nil stack to arbitrary ones *)
+Definition liftNilRel (R : Rel (FunStackE E1 pnil) (FunStackE E2 pnil)) :
+  Rel (FunStackE E1 stk1) (FunStackE E2 stk2) :=
+  fun e1 e2 => match e1,e2 with
+               | inr e1', inr e2' => R (inr e1') (inr e2')
+               | _,_ => False
+               end.
+
+(* Lift a postcondition on FunStackE events from the nil stack to arbitrary ones *)
+Definition liftNilPostRel (R : PostRel (FunStackE E1 pnil) (FunStackE E2 pnil)) :
+  PostRel (FunStackE E1 stk1) (FunStackE E2 stk2) :=
+  fun e1 e2 => match e1,e2 with
+               | inr e1', inr e2' => R (inr e1') (inr e2')
+               | _,_ => fun _ _ => False
+               end.
+
+Lemma observing_LetRecS E R stk funs body :
+  LetRecS E R stk funs body = LetRecS E R stk funs (go _ _ (observe body)).
+Proof.
+  reflexivity.
+Qed.
+
+Lemma observing_BindS E stk A B m (k : A -> SpecM E stk B) :
+  BindS m k = BindS (go _ _ (observe m)) k.
+Proof.
+  reflexivity.
+Qed.
+
+(* lr_refines is sound, meaning that it implies two letrecs refine each other *)
+Lemma lr_refines_soundness RPre RPost t1 t2 :
+  lr_refines funs1 funs2 (liftNilRel RPre) (liftNilPostRel RPost) RR t1 t2 ->
+  refines RPre RPost RR (LetRecS _ R1 _ funs1 t1) (LetRecS _ R2 _ funs2 t2).
+Proof.
+  revert t1 t2; pcofix CIH; intros.
+  rewrite observing_LetRecS. rewrite (observing_LetRecS E2).
+  punfold H0. red in H0. pstep. red.
+  unfold SpecM, FunStackE, EncodingType_FunStackE in * |- *.
+  remember (observe t1) as ot1.
+  remember (observe t2) as ot2.
+  clear t1 Heqot1 t2 Heqot2.
+  hinduction H0 before r; intros; pclearbot; eauto.
+  - constructor; assumption.
+  - apply refinesF_Tau. right. apply CIH. apply H.
+  - unfold liftNilRel in H.
+    destruct e1; [ contradiction | ]. destruct e2; [ contradiction | ].
+    cbn. eapply refinesF_Vis; [ apply H | ].
+    intros. right. apply CIH.
+    destruct (H0 a b H1); [ | destruct H2 ]. apply H2.
+  - cbn. apply refinesF_TauL. apply IHlr_refinesF. intros. apply CIH. assumption.
+  - cbn. apply refinesF_TauR. apply IHlr_refinesF. intros. apply CIH. assumption.
+  - cbn. apply refinesF_forallR. intros. apply H0. intros. apply CIH. assumption.
+  - cbn. eapply refinesF_existsR. apply IHlr_refinesF.
+    intros. apply CIH. assumption.
+  - cbn. eapply refinesF_forallL. apply IHlr_refinesF.
+    intros. apply CIH. assumption.
+  - cbn. apply refinesF_existsL. intros. apply H0. intros. apply CIH. assumption.
+Qed.
+
+(* lr_refines is complete, meaning that it holds whenever two letrecs refine
+each other *)
+Lemma lr_refines_completeness RPre RPost t1 t2 t1' t2' :
+  observe t1' = observe (LetRecS _ R1 _ funs1 t1) ->
+  observe t2' = observe (LetRecS _ R2 _ funs2 t2) ->
+  refines RPre RPost RR t1' t2' ->
+  lr_refines funs1 funs2 (liftNilRel RPre) (liftNilPostRel RPost) RR t1 t2.
+Proof.
+  revert t1 t2 t1' t2'; pcofix CIH; intros.
+  punfold H2. red in H2. pstep. red.
+  remember (observe t1') as ot1'. remember (observe t2') as ot2'.
+  clear t1' Heqot1' t2' Heqot2'.
+  hinduction H2 before r; intros; pclearbot; eauto.
+  - destruct t1 as [[]]; destruct t2 as [[]]; try discriminate.
+    + injection H0; intros; injection H1; intros. constructor.
+      subst r1. subst r2. assumption.
+    + admit.
+Admitted.
+
+
+(* Add a precondition for recursive calls *)
+Definition addCallPreRel {E1 E2 : EncType} {stk1 stk2}
+           (precond : Rel (FrameCall stk1) (FrameCall stk2))
+           (RPre : Rel (FunStackE E1 pnil) (FunStackE E2 pnil)) :
+  Rel (FunStackE E1 stk1) (FunStackE E2 stk2) :=
+  fun a1 a2 => match a1,a2 with
+               | inl args1, inl args2 => precond args1 args2
+               | inr ev1, inr ev2 => RPre (inr ev1) (inr ev2)
+               | _, _ => False
+               end.
+
+(* Add a postcondition for recursive calls *)
+Definition addCallPostRel {E1 E2 : EncType} {stk1 stk2}
+           (postcond : PostRel (FrameCall stk1) (FrameCall stk2))
+           (RPost : PostRel (FunStackE E1 pnil) (FunStackE E2 pnil)) :
+  PostRel (FunStackE E1 stk1) (FunStackE E2 stk2) :=
+  fun a1 a2 => match a1,a2 with
+               | inl args1, inl args2 => postcond args1 args2
+               | inr ev1, inr ev2 => RPost (inr ev1) (inr ev2)
+               | _, _ => fun _ _ => False
+               end.
+
+
+Lemma lr_refines_bind RPre RPost S1 S2 (RS : Rel S1 S2) m1 m2 k1 k2 :
+  lr_refines funs1 funs2 RPre RPost RS m1 m2 ->
+  (forall x1 x2, RS x1 x2 ->
+                 lr_refines funs1 funs2 RPre RPost RR (k1 x1) (k2 x2)) ->
+  lr_refines funs1 funs2 RPre RPost RR (m1 >>= k1) (m2 >>= k2).
+Proof.
+  intros mref kref; revert m1 m2 mref; pcofix CIH; intros.
+  punfold mref; red in mref.
+  rewrite (observing_BindS E1). rewrite (observing_BindS E2).
+  unfold EncodingType_FrameCall, encodes.
+  remember (observe m1) as om1. remember (observe m2) as om2.
+  clear m1 m2 Heqom1 Heqom2.
+  hinduction mref before om1; intros; pclearbot.
+  - eapply paco2_mon.
+    + setoid_rewrite bind_ret_l. apply kref; assumption.
+    + intros. destruct PR.
+  - pstep. apply lr_refinesF_Tau. right. apply CIH. assumption.
+  - pstep. apply lr_refinesF_Vis; [ assumption | ].
+    intros. right. apply CIH. remember (H0 a b H1).
+    destruct u; [ assumption | destruct b0 ].
+  - pstep. apply lr_refinesF_TauL. pstep_reverse.
+  - pstep. apply lr_refinesF_TauR. pstep_reverse.
+  - pstep. apply lr_refinesF_forallR. intros. pstep_reverse. apply H0.
+  - pstep. eapply lr_refinesF_existsR. pstep_reverse. apply IHmref.
+  - pstep. eapply lr_refinesF_forallL. pstep_reverse. apply IHmref.
+  - pstep. apply lr_refinesF_existsL. intros. pstep_reverse. apply H0.
+  - pstep. setoid_rewrite bind_vis. apply lr_refinesF_unfoldL.
+    change
+      (lr_refinesF funs1 funs2 RPre RPost RR
+         (upaco2 (lr_refines_ funs1 funs2 RPre RPost RR) r)
+         (observe (Tau (x <- applyFrameTuple E1 stk1 funs1 call1;; EnTree.bind (k0 x) k1)))
+         (observe (x <- {| _observe := ot2 |};; k2 x))).
+    pstep_reverse. 
+    setoid_rewrite <- bind_tau. setoid_rewrite <- bind_bind.
+    apply IHmref.
+  - pstep. setoid_rewrite bind_vis. apply lr_refinesF_unfoldR.
+    change
+      (lr_refinesF funs1 funs2 RPre RPost RR
+         (upaco2 (lr_refines_ funs1 funs2 RPre RPost RR) r)
+         (observe (x <- {| _observe := ot1 |};; k1 x))
+         (observe (Tau (x <- applyFrameTuple E2 stk2 funs2 call2;; EnTree.bind (k0 x) k2)))).
+    pstep_reverse.
+    setoid_rewrite <- bind_tau. setoid_rewrite <- bind_bind.
+    apply IHmref.
+Qed.
+
+
+(* We can discharge a local assumption about calls if it holds for the calls *)
+Lemma lr_refines_discharge RPre RPost precond postcond t1 t2 :
+  (forall call1 call2,
+      (precond call1 call2 : Prop) ->
+      lr_refines funs1 funs2 (addCallPreRel precond RPre)
+        (addCallPostRel postcond RPost) (postcond call1 call2)
+        (applyFrameTuple _ _ funs1 call1)
+        (applyFrameTuple _ _ funs2 call2)) ->
+  lr_refines funs1 funs2 (addCallPreRel precond RPre)
+    (addCallPostRel postcond RPost) RR t1 t2 ->
+  lr_refines funs1 funs2 (liftNilRel RPre) (liftNilPostRel RPost) RR t1 t2.
+Proof.
+  intro funsRef. revert t1 t2; pcofix CIH; intros.
+  punfold H0. red in H0. pstep. red.
+  remember (observe t1) as ot1.
+  remember (observe t2) as ot2.
+  clear t1 Heqot1 t2 Heqot2.
+  hinduction H0 before ot1; intros; pclearbot.
+  - apply lr_refinesF_Ret. assumption.
+  - apply lr_refinesF_Tau. right. apply CIH. apply H.
+  - destruct e1; destruct e2.
+    + apply lr_refinesF_unfoldL. apply lr_refinesF_unfoldR.
+      apply lr_refinesF_Tau. right. apply CIH.
+      apply (lr_refines_bind _ _ _ _ (postcond f f0)).
+      -- apply funsRef. assumption.
+      -- intros. destruct (H0 x1 x2 H1) as [ H3 | [] ].
+         assumption.
+    + destruct H.
+    + destruct H.
+    + apply lr_refinesF_Vis; [ apply H | ]. intros.
+      right. apply CIH. destruct (H0 a b H1) as [ H2 | [] ].
+      assumption.
+  - apply lr_refinesF_TauL. assumption.
+  - apply lr_refinesF_TauR. assumption.
+  - apply lr_refinesF_forallR. intros. apply H0.
+  - eapply lr_refinesF_existsR. apply IHlr_refinesF.
+  - eapply lr_refinesF_forallL. apply IHlr_refinesF.
+  - apply lr_refinesF_existsL. intros. apply H0.
+  - apply lr_refinesF_unfoldL. apply IHlr_refinesF.
+  - apply lr_refinesF_unfoldR. apply IHlr_refinesF.
+Qed.
+
+End lr_refines_props.
